src/assign_mcl.lean
@@ -26,13 +26,19 @@ end
 
 def p₁ : mclp sig := mclp.intro (λ m, 100) (
     mclk.global_assign "a" [read_tid] (by refl) (by refl) read_tid ;;
-    mclk.global_assign "b" [read_tid] (by refl) (by refl) (read_tid + 1)
+    mclk.global_assign "b" [read_tid] (by refl) (by refl) (read_tid + (expression.const_int 1 (by refl)))
 )
 
 def p₂ : mclp sig := mclp.intro (λ m, 100) (
-    mclk.global_assign "b" [read_tid] (by refl) (by refl) (read_tid + 1) ;;
+    mclk.global_assign "b" [read_tid] (by refl) (by refl) (read_tid + (expression.const_int 1 (by refl))) ;;
     mclk.global_assign "a" [read_tid] (by refl) (by refl) read_tid
 )
+
+open parlang
+open parlang.state
+open parlang.thread_state
+
+#reduce update_global_vars_for_expr (read_tid + 1)
 
 -- this approach is like computing both programs and comparing their output
 -- this is a fairly naive approach, another approach would be to show that their behavior is equal (based on the fact that we have to show equality)
@@ -64,9 +70,49 @@ example : mclp_rel eq p₁ p₂ eq := begin
     cases h with m₁ h,
     cases h with m₂ h,
     simp,
-    -- todo: we need ways to reason about ranges of memory
+    have : n₁ = n₂ := begin
+        sorry
+    end,
+    subst this,
+    have hseq : s₁ = s₂ := begin
+        sorry
+    end,
+
+    -- the proof obligation in the form of a map thread on syncable is the simple version because we never consider threads to change active state (here all threads are always active)
+
+    -- h expresses the initial state (we might want to compress this information)
+    -- todo: we need ways to reason about ranges of memory (dependent on tid, ergo n₁)
     -- e.g. using foldr
-    apply exists.intro (m₁.update ("a", [0]) (7 : ℕ)),
+    apply exists.intro ((list.range n₁).foldl (λ (m : parlang.memory (parlang_mcl_global sig)) i, ((memory.update ("b", [i]) (i + 1 : ℕ) ∘ (memory.update ("a", [i]) i))) m) m₁),
+    
+    split, {
+        have : update_global_vars_for_expr read_tid = id := by refl,
+        rw this,
+        have : update_global_vars_for_expr (read_tid + (expression.const_int 1 (show type_of (sig "b") = type_of (sig "b"), by refl))) = id := by refl,
+        rw this,
+        simp,
+
+        -- put maps in store
+        rw ← function.comp.assoc,
+        rw ← function.comp.assoc,
+        rw thread_state_map,
+        rw ← function.comp.assoc,
+        rw thread_state_map',
+        rw function.comp.assoc,
+        rw function.comp.assoc,
+        rw syncable_remove_map,
+        
+        rw ← function.comp.assoc,
+        rw thread_state_map',
+        rw function.comp.assoc,
+        rw syncable_remove_map,
+        
+        simp,
+        -- resolve get and update (the result should only be mcl_init, literals and memory (in case of loads))
+        -- only stores left
+        -- find a way to resolve the stores all together
+    }
+
 end
 
 end assign_mcl
